eval
git-svn-id: svn://scm.gforge.inria.fr/svn/cfml@197 ba02c806-7d2b-4818-9a48-35b22e6bdc79

imper/LambdaEval_proof.v
@@ -4,7 +4,7 @@
 ***************************************************************************)
 
 Set Implicit Arguments.
-Require Import CFPrim VerifEval_ml.
+Require Import CFPrim LambdaEval_ml.
 
 
 (*==========================================================*)
@@ -14,11 +14,11 @@ Require Import CFPrim VerifEval_ml.
 (************************************************************)
 (* ** Specification of substitution *)
 
-Fixpoint Subst (x : int) (v : Term) (t : Term) {struct t} : Term :=
+Fixpoint Subst (x : int) (v : term) (t : term) : term :=
   match t with
-  | Tvar y => if x == y then v else t
+  | Tvar y => if x '= y then v else t
   | Tint n => Tint n
-  | Tfun y b => Tfun y (if x == y then b else Subst x v b)
+  | Tfun y b => Tfun y (if x '= y then b else Subst x v b)
   | Tapp t1 t2 => Tapp (Subst x v t1) (Subst x v t2)  
   end.
 
@@ -26,7 +26,7 @@ Fixpoint Subst (x : int) (v : Term) (t : Term) {struct t} : Term :=
 (************************************************************)
 (* ** Specification of big-step reduction *)
 
-Inductive Reds : Term -> Term -> Prop :=
+Inductive Reds : term -> term -> Prop :=
   | Reds_int : forall n,
       Reds (Tint n) (Tint n)
   | Reds_fun : forall y b,
@@ -40,54 +40,150 @@ Inductive Reds : Term -> Term -> Prop :=
 (************************************************************)
 (* ** Subterm relationship, to argue for termination *)
 
-Inductive Term_sub : Term -> Term -> Prop :=
-  | Term_sub_fun : forall x t,
-     Term_sub t (Tfun x t)
-  | Term_sub_app_1 : forall t1 t2,
-     Term_sub t1 (Tapp t1 t2) 
-  | Term_sub_app_2 : forall t1 t2,
-     Term_sub t2 (Tapp t1 t2).
+Inductive term_sub : term -> term -> Prop :=
+  | term_sub_fun : forall x t,
+     term_sub t (Tfun x t)
+  | term_sub_app_1 : forall t1 t2,
+     term_sub t1 (Tapp t1 t2) 
+  | term_sub_app_2 : forall t1 t2,
+     term_sub t2 (Tapp t1 t2).
   
-Hint Constructors Term_sub.
+Hint Constructors term_sub.
 
-Lemma Term_sub_wf : well_founded Term_sub.
+Lemma term_sub_wf : wf term_sub.
 Proof.
   intros t. induction t; apply Acc_intro;
     introv H; inverts H; auto.
 Qed.
 
-Hint Resolve Term_sub_wf : wf.
+Hint Resolve term_sub_wf : wf.
 
 
 (*==========================================================*)
 (* * Verification of the code *)
 (*==========================================================*)
 
+Tactic Notation "xintros" simple_intropattern(x1) :=
+  xintros; intros x1.
+Tactic Notation "xintros" simple_intropattern(x1) simple_intropattern(x2) :=
+  xintros; intros x1 x2.
+Tactic Notation "xintros" simple_intropattern(x1) simple_intropattern(x2)
+  simple_intropattern(x3) :=
+  xintros; intros x1 x2 x3.
+Tactic Notation "xintros" simple_intropattern(x1) simple_intropattern(x2)
+  simple_intropattern(x3) simple_intropattern(x4) :=
+  xintros; intros x1 x2 x3 x4.
+
+Tactic Notation "xrets" :=
+  xret; xsimpl.
+Tactic Notation "xrets" "~" :=
+  xrets; xauto~.
+Tactic Notation "xapps" "~" :=
+  xapps; xauto~.
+
+(*todo:remove*)
+Ltac xapps_core spec args solver ::=
+  let cont1 tt :=
+    xapp_with spec args solver in
+  let cont2 tt :=
+    instantiate; xextract; try intro_subst in    
+  match ltac_get_tag tt with
+  | tag_let_trm => xlet; [ cont1 tt | cont2 tt ]
+  | tag_seq =>     xseq; [ cont1 tt | cont2 tt ]
+  end.
+
+Tactic Notation "xlets" constr(Q) :=
+  xlet Q; [ | intro_subst ].
+
 Lemma subst_spec :
-  spec subst [x:_Int] [v:_Term] [t:_Term] 
-    is >> _Term st = Subst x v t.
+  Spec subst x v t |R>> R [] \[= Subst x v t].
 Proof.
-  xinduction (unproj33 int Term Term_sub).
-  xintros x v t. intros IH. xred. 
-  destruct t as [ y | n | y b | t1 t2]; xpat.
-    xapplys. xcase as H; simpl.
-      xreturns. rewriteb~ H.
-      #xreturns. rewriteb~ H.
-    #xreturns.
-    xapplys. xcase as H; simpl.
-      #xreturns. rewriteb~ H.
-      xapplys~. #xreturns. rewriteb~ H.
-    xapplys~. xapplys~. #xreturns.
+  xinduction (unproj33 int term term_sub). 
+  xintros x v t. intros IH. 
+  apply app_spec_3. xcf. intro_subst_arity 3%nat.  (* todo : tactic *)
+  xmatch; simpl. (* destruct t as [ y | n | y b | t1 t2] *)
+  destruct (x '= y); xif; xrets~. (* todo: better *) 
+  xrets~.
+  xlets (\[ = (if x '= y then b else Subst x v b) ]). (* todo: auto *)
+    xif.
+      xrets. case_if~. false.
+      xapps~. xrets~. case_if~. false.
+   xrets~.
+  xapps~. xapps~. xrets~.
 Qed.
 
+Hint Extern 1 (RegisterSpec subst) => Provide subst_spec.
+
+
+Lemma app_weaken_1 : forall B H1 Q1 H2 A1 (x1:A1) f H (Q:B->hprop),
+  app_1 f x1 H1 Q1 -> 
+  H ==> H1 \* H2 -> 
+  Q1 \*+ H2 ===> Q ->
+  app_1 f x1 H Q.
+Proof. intros. applys* local_wframe. Qed.
+
+Lemma app_weaken_2 : forall B H1 Q1 H2 A1 A2 (x1:A1) (x2:A2) f H (Q:B->hprop),
+  app_2 f x1 x2 H1 Q1 -> 
+  H ==> H1 \* H2 -> 
+  Q1 \*+ H2 ===> Q ->
+  app_2 f x1 x2 H Q.
+Proof. intros. applys* local_wframe. Qed.
+
+Lemma app_weaken_3 : forall B H1 Q1 H2 A1 A2 A3 (x1:A1) (x2:A2) (x3:A3) f H (Q:B->hprop),
+  app_3 f x1 x2 x3 H1 Q1 -> 
+  H ==> H1 \* H2 -> 
+  Q1 \*+ H2 ===> Q ->
+  app_3 f x1 x2 x3 H Q.
+Proof. intros. applys* local_wframe. Qed.
+
+Lemma app_weaken_4 : forall B H1 Q1 H2 A1 A2 A3 A4 (x1:A1) (x2:A2) (x3:A3) (x4:A4) f H (Q:B->hprop),
+  app_4 f x1 x2 x3 x4 H1 Q1 -> 
+  H ==> H1 \* H2 -> 
+  Q1 \*+ H2 ===> Q ->
+  app_4 f x1 x2 x3 x4 H Q.
+Proof. intros. applys* local_wframe. Qed.
+
+Ltac get_app_weaken_x x :=
+  match x with
+     | 1%nat => constr:(app_weaken_1)
+     | 2%nat => constr:(app_weaken_2)
+     | 3%nat => constr:(app_weaken_3)
+     | 4%nat => constr:(app_weaken_4)
+  end.
+
+
+          
+Ltac try_app_hyp f cont :=
+  match goal with
+  | H: context [ app_1 f _ _ _ ] |- _ => cont (H)
+  | H: context [ app_2 f _ _ _ _ ] |- _ => cont (H)
+  | H: context [ app_3 f _ _ _ _ _ ] |- _ => cont (H) 
+  | H: context [ app_4 f _ _ _ _ _ _ ] |- _ => cont (H) 
+  end.
+
+Tactic Notation "xapp'" :=
+  xuntag tag_apply; 
+  let f := spec_goal_fun tt in 
+  try_app_hyp f ltac:(fun H =>
+  (*let n := spec_term_arity H in*)
+  let n := spec_goal_arity tt in
+  let W := get_app_weaken_x n in
+  eapply W; [ apply H | hsimpl | try apply rel_le_refl ]).
+
+Tactic Notation "xapps'" :=
+  xlet; [ xapp' | try xextract; try intro_subst ].
+
 Lemma eval_spec :
-  spec eval [t:_Term] = r is
-    forall v, Reds t v -> r >> _Term st = v.
+  Spec eval t |R>> forall v, Reds t v -> R [] (\= v).
 Proof.
-  introv Red. induction Red; xred; xpat.
-    #xreturns.
-    #xreturns. 
-    xinouts~. xreds 2. xinouts~. xapplys~ subst_spec. 
+  xintros t. introv Red. induction Red;
+  apply app_spec_1; xcf; intro_subst_arity 1%nat; 
+  xmatch.  (* todo : tactic *)
+  xrets~.
+  xrets~.
+  xapps'. xmatch; [ | false* C0 ]. (* tactic todo *)
+  xapps'.
+  xapps. xapp'. xsimpl~.
 Qed.
 
 
